Started Exercise 4

P1/Ex4.dfy
@@ -9,12 +9,41 @@ import Ex3=Ex3
 class Queue {
 
   var lst1 : Ex3.Node?
-  var lst2 : Ex3.Node? 
+  var lst2 : Ex3.Node?
+
+  ghost var list1: multiset<int>
+  ghost var list2: multiset<int>
+
+  ghost var footprint1: set<Ex3.Node>
+  ghost var footprint2: set<Ex3.Node>
 
   // Ex1
-  ghost function Valid() : bool 
+  ghost function Valid() : bool
+    reads 
+      this,
+      lst1, 
+      lst2, 
+      if lst1 == null then {} else lst1.footprint,
+      if lst2 == null then {} else lst2.footprint
   {
-    // ToDo  
+    (lst1 != null ==>
+      this.footprint1 == lst1.footprint &&
+      lst1.Valid() &&
+      list1 == multiset(lst1.list)
+    ) &&
+    (lst1 == null ==>
+      this.footprint1 == {} &&
+      list1 == multiset{}
+    ) &&
+    (lst2 != null ==>
+      this.footprint2 == lst2.footprint &&
+      lst2.Valid() &&
+      list2 == multiset(lst2.list)
+    ) &&
+    (lst2 == null ==>
+      this.footprint2 == {} &&
+      list2 == multiset{}
+    )
   }
 
   // Ex2 
@@ -22,28 +51,44 @@ class Queue {
   {
     this.lst1 := null; 
     this.lst2 := null;  
-    // ToDo
+    this.footprint1 := {};
+    this.footprint2 := {};
+    this.list1 := multiset{};
+    this.list2 := multiset{};
   } 
 
   // Ex3.1
-  method push(val : int) 
+  method push(val : int)
+    requires Valid()
+    ensures Valid()
+    modifies this, this.footprint1
   {
-    lst1 := Ex3.ExtendList(lst1, val);     
+    lst1 := Ex3.ExtendList(lst1, val);
+    this.list1 := multiset(lst1.list);
+    this.footprint1 := lst1.footprint;
   }
 
   // Ex3.2
   method pop() returns (r : int)
+    requires Valid() && lst1 != null
+    ensures Valid()
+    modifies this, this.footprint2, this.footprint1
   {
 
     if (lst2 == null) {
       lst2 := lst1.reverse(null); 
       lst1 := null;
+      footprint1 := {};
+      footprint2 := lst2.footprint;
+      list1 := multiset{};
+      list2 := multiset(lst2.list);
     }
 
-    r := lst2.data; 
-    lst2 := lst2.next; 
+    r := lst2.data;
+    footprint2 := footprint2 - {lst2};
+    list2 := list2 - multiset([lst2.data]);
+    lst2 := lst2.next;
   }
-  
 }
 
 }
